steel/Zeta.Correctness.fst
@@ -1,0 +1,29 @@
+module Zeta.Correctness
+open Zeta.Steel.ThreadStateModel
+
+// There's a bunch of old code/proofs in
+// to_be_restored/Veritas.SingleThreadSimulation
+// that could help with this proof
+// The main lemma there, related_entries, says that if you
+// start the Veritas.Steel.ThreadStateModel and
+// Intermediate.Verifier in related stats
+// and you run them on related log entries
+// then they end in related states.
+// But, those definitions are stale
+
+assume
+val seq_consistent (logs:all_logs) (eid:epoch_id)
+  : prop
+
+assume
+val merkle_hash_collision : Type0
+
+assume
+val multiset_hash_collision : Type0
+
+(* the definition of epoch_is_certified may need to be adjusted ... *)
+let main_lemma (logs:all_logs)
+               (eid:epoch_id { epoch_is_certified logs eid })
+               (_ : squash (~ (seq_consistent logs eid) ))
+  : Tot (either merkle_hash_collision multiset_hash_collision)
+  = admit()
