steel/Zeta.Steel.VerifierTypes.fsti
@@ -1,0 +1,50 @@
+module Zeta.Steel.VerifierTypes
+
+open FStar.Ghost
+open Zeta.Steel.ApplicationTypes
+module U8 = FStar.UInt8
+module U16 = FStar.UInt16
+module U32 = FStar.UInt32
+module U64 = FStar.UInt64
+open Zeta.Steel.FormatsManual
+open Steel.Memory
+open Steel.Effect.Atomic
+open Steel.Effect
+open Steel.Reference
+open Steel.Array
+
+module T = Zeta.Steel.FormatsManual
+module M = Zeta.Steel.ThreadStateModel
+module A = Steel.Array
+module AEH = Zeta.Steel.AggregateEpochHashes
+
+#push-options "--ide_id_info_off"
+
+val thread_state_t
+  : Type0
+
+noextract
+val thread_state_inv (t:thread_state_t)
+  : vprop
+
+val type_of_thread_state_inv (t:thread_state_t) :
+  Lemma (ensures (t_of (thread_state_inv t)) == M.thread_state_model)
+        [SMTPat (t_of (thread_state_inv t))]
+
+let coerce_eq (#a:Type) (#b:Type) (_:squash (a == b)) (x:a) : b = x
+let value_of (t:thread_state_t) ($r:rmem (thread_state_inv t))
+  : GTot M.thread_state_model
+  = type_of_thread_state_inv t;
+    coerce_eq () (r (thread_state_inv t))
+
+val elim_thread_state_inv (#o:_) (t:thread_state_t)
+  : SteelGhost unit o
+    (thread_state_inv t)
+    (fun _ -> thread_state_inv t)
+    (requires fun h0 -> True)
+    (ensures fun h0 _ h1 ->
+      let tsm0 = value_of t h0 in
+      let tsm1 = value_of t h1 in
+      tsm0 == tsm1 /\
+      tsm1 == M.verify_model (M.init_thread_state_model tsm1.thread_id)
+                             tsm1.processed_entries)
