steel/code_structure.md
@@ -1,0 +1,84 @@
+In rough dependence order
+
+### Zeta.Steel.Parser
+
+Tahina owns.
+
+It represents a kind of minimalistic port of LowParse
+
+### Zeta.ApplicationTypes.fsti
+
+The main spec-level interface to be defined by the application. It's
+opened by nearly all other modules.
+
+### Zeta.Steel.FormatsManual
+
+Tahina owns.
+
+It sets the log format. Probably to be replaced with an auto-generated one.
+
+It also provides signatures for some parsers and serializers of app
+and stamped records. These could be moved somewhere else
+
+### Zeta.Steel.KeyUtils
+
+Some simple utilities on internal keys
+
+### Zeta.Steel.ThreadStateModel
+
+Nik and Arvind share this one.
+
+The main specification of a Steel verifier thread.
+
+Defines the `thread_state_model` type.
+
+### Zeta.Steel.Correctness
+
+Arvind owns.
+
+It related ThreadStateModel to Zeta.Intermediate.Verifier and provides
+the main semantic correctness lemma.
+
+### Zeta.Steel.VerifierTypes
+
+Defines the concrete type of a verifier's thread state,
+`thread_state_t`
+
+And an invariant on that state `thread_state_inv`.
+
+And a selector that allows reading a `thread_state_t` as a
+`thread_state_model` for specification.
+
+### Zeta.Steel.Application.fsti
+
+Defines the signature of `run_app_function`, which must be implemented
+by an application instance. The spec relates it to
+ThreadStateModel.run_app.
+
+### Zeta.Steel.AggregateEpochHashes.fsti
+
+Defines the type `aggregate_epoch_hashes` and an invariant associated
+with it. It type is a record that holds a reference to the global
+epoch hashes and max_certified epoch. Both are protected by a single
+lock.
+
+### Zeta.Steel.Verifier.fsti
+
+Nik own this one.
+
+The Steel implementation of a verifier thread. Its main function is
+`verify_entries`, which takes an input log, and output array, an
+aggregate_epoch_hashes, and verifies it according the to spec given in
+ThreadStateModel.
+
+### Zeta.Steel.Main.fsti
+
+Aseem owns this one.
+
+The top-level interface, providing `verify_entries` and `max_certified_epoch`
+
+
+### Other files
+
+HashAccumulator + some files in `to_be_restored` are kind of leaves in
+the develpoment.
